ulib/FStar.Relational.Comp.fst
@@ -11,23 +11,23 @@ let st2_Post (a:Type) = st_post_h heap2 a
 let st2_WP (a:Type) = st_wp_h heap2 a
 effect ST2 (a:Type) (pre:st2_Pre) (post: (heap2 -> Tot (st2_Post a))) =
     STATE2 a
-      (fun (p:st2_Post a) (h:heap2) -> pre h /\ (forall a h1. pre h /\ post h a h1 ==> p a h1)) (* WP *)
+      (fun (is_wlp:bool) (p:st2_Post a) (h:heap2) -> (is_wlp \/ pre h) /\ (forall a h1. pre h /\ post h a h1 ==> p a h1)) (* WP *)
 effect St2 (a:Type) = ST2 a (fun h -> True) (fun h0 r h1 -> True)
 sub_effect
-  DIV    ~> STATE2 = (fun (a:Type) (wp:pure_wp a) (p:st2_Post a) -> (fun h2 -> wp (fun a0 -> p a0 h2)))
+  DIV    ~> STATE2 = (fun (a:Type) (wp:pure_wp a) (is_wlp:bool) (p:st2_Post a) -> (fun h2 -> wp is_wlp (fun a0 -> p a0 h2)))
 
 (* construct a st2_WP from 2 st_wps *)
 val comp : (a:Type) -> (b:Type) -> (wp0:st_wp a) -> (wp1:st_wp b) -> Tot (st2_WP (rel a b)) 
-let comp a b wp0 wp1 p h2 =
-    wp0 (fun y0 h0 ->
-      wp1 (fun y1 h1 -> p (R y0 y1) (R h0 h1))
+let comp a b wp0 wp1 is_wlp p h2 =
+    wp0 is_wlp (fun y0 h0 ->
+      wp1 is_wlp (fun y1 h1 -> p (R y0 y1) (R h0 h1))
       (R.r h2))
     (R.l h2)
 
 //TODO: this should be conditional on the monotonicity of the wps
-assume Monotone_comp: forall a b wp1 wp2 p1 p2. (forall x h. p1 x h ==> p2 x h)
-			==> (forall h. comp a b wp1 wp2 p1 h
-			    ==> comp a b wp1 wp2 p2 h)
+assume Monotone_comp: forall a b wp1 wp2 is_wlp p1 p2. (forall x h. p1 x h ==> p2 x h)
+			==> (forall h. comp a b wp1 wp2 is_wlp p1 h
+			    ==> comp a b wp1 wp2 is_wlp p2 h)
 
 
 assume val compose2: #a0:Type -> #b0:Type -> #wp0:(a0 -> Tot (st_wp b0))
@@ -71,17 +71,17 @@ assume val cross : #a:Type -> #b:Type -> #c:Type -> #d:Type
 val decomp_l : (a0:Type) -> (a1:Type) -> (b0:Type) -> (b1:Type) -> (al:a0) -> (wp:(rel a0 a1 -> Tot (st2_WP (rel b0 b1))))
 	     -> Tot (st_wp_h heap b0)
 let decomp_l a0 a1 b0 b1 al wp =
-  fun p hl ->
+  fun is_wlp p hl ->
     (exists (ar:a1) (hr:heap).
-      wp (R al ar) (fun y2 h2 -> p (R.l y2) (R.l h2))
+      wp  (R al ar) is_wlp (fun y2 h2 -> p (R.l y2) (R.l h2))
          (R hl hr))
 
 val decomp_r : (a0:Type) -> (a1:Type) -> (b0:Type) -> (b1:Type) -> (ar:a1) -> (wp:(rel a0 a1 -> Tot (st2_WP (rel b0 b1))))
 	     -> Tot (st_wp_h heap b1)
 let decomp_r a0 a1 b0 b1 ar wp =
-  fun p hr ->
+  fun is_wlp p hr ->
     (exists (al:a0) (hl:heap).
-      wp (R al ar) (fun y2 h2 -> p (R.r y2) (R.r h2))
+      wp (R al ar) is_wlp (fun y2 h2 -> p (R.r y2) (R.r h2))
          (R hl hr))
 
 assume val project_l : #a0:Type -> #b0:Type -> #a1:Type -> #b1:Type
