ulib/prims.fst
@@ -102,33 +102,41 @@ type range_of (#a:Type) (x:a) = range
 (* PURE effect *)
 let pure_pre = Type0
 let pure_post (a:Type) = a -> GTot Type0
-let pure_wp   (a:Type) = pure_post a -> GTot pure_pre
+let pure_wp   (a:Type) = bool -> pure_post a -> GTot pure_pre
 
-inline let pure_return (a:Type) (x:a) (p:pure_post a) =
+inline let pure_return (a:Type) (x:a) (is_wlp:bool) (p:pure_post a) =
      p x
 
 inline let pure_bind_wp (r1:range) (a:Type) (b:Type)
                    (wp1:pure_wp a) (wp2: (a -> GTot (pure_wp b)))
-                   (p : pure_post b) =
+                   (is_wlp:bool) (p : pure_post b) =
      labeled r1 "push" unit 
-     /\ wp1 (fun (x:a) -> 
+     /\ wp1 is_wlp (fun (x:a) -> 
              labeled r1 "pop" unit 
-	     /\ wp2 x p)
-inline let pure_if_then_else (a:Type) (p:Type) (wp_then:pure_wp a) (wp_else:pure_wp a) (post:pure_post a) =
-     l_ITE p (wp_then post) (wp_else post)
+	     /\ wp2 x is_wlp p)
+inline let pure_if_then_else (a:Type) (p:Type) (wp_then:pure_wp a) (wp_else:pure_wp a) (is_wlp:bool) (post:pure_post a) =
+     l_ITE p (wp_then is_wlp post) (wp_else is_wlp post)
 
-inline let pure_ite_wp (a:Type) (wp:pure_wp a) (post:pure_post a) =
-     (forall (x:a). ~(wp (fun (x':a) -> ~(eq2 #a #a x x'))) ==> post x)
-     /\ wp (fun _ -> True)
+assume type guard_free : Type0 -> Type0
 
-inline let pure_wp_binop (a:Type) (wp1:pure_wp a) (op:(Type -> Type -> GTot Type)) (wp2:pure_wp a) (p:pure_post a) =
-     op (wp1 p) (wp2 p)
-inline let pure_wp_as_type (a:Type) (wp:pure_wp a) = forall (p:pure_post a). wp p
-inline let pure_close_wp (a:Type) (b:Type) (wp:(b -> GTot (pure_wp a))) (p:pure_post a) = forall (b:b). wp b p
-inline let pure_assert_p (a:Type) (q:Type) (wp:pure_wp a) (p:pure_post a) = q /\ wp p
-inline let pure_assume_p (a:Type) (q:Type) (wp:pure_wp a) (p:pure_post a) = q ==> wp p
-inline let pure_null_wp  (a:Type) (p:pure_post a) = forall (x:a). p x
-inline let pure_trivial  (a:Type) (wp:pure_wp a) = wp (fun (x:a) -> True)
+(* inline let pure_ite_wp (a:Type) (wp:pure_wp a) (is_wlp:bool) (post:pure_post a) = *)
+(*    forall (wp_proxy:bool -> (a -> Type0) -> Type0). *)
+(*         (forall (flag:bool) (q:(a -> Type)).{:pattern (guard_free (wp_proxy flag q))} wp_proxy flag q <==> wp flag q) //pick a name wp_proxy for wp *)
+(*     ==> ((forall (x:a). ~(wp_proxy true (fun (x':a) -> ~(eq2 #a #a x x'))) ==> post x) //and use wp_proxy once here *)
+(*          /\ (is_wlp \/ wp_proxy false (fun _ -> True))) //and another time here *)
+
+inline let pure_ite_wp (a:Type) (wp:pure_wp a) (is_wlp:bool) (post:pure_post a) =
+     (forall (x:a). ~(wp true (fun (x':a) -> ~(eq2 #a #a x x'))) ==> post x)
+     /\ (is_wlp \/ wp false (fun _ -> True))
+
+inline let pure_wp_binop (a:Type) (wp1:pure_wp a) (op:(Type -> Type -> GTot Type)) (wp2:pure_wp a) (is_wlp:bool) (p:pure_post a) =
+     op (wp1 is_wlp p) (wp2 is_wlp p) 
+inline let pure_wp_as_type (a:Type) (wp:pure_wp a) = forall (p:pure_post a). wp false p //TODO: WHAT SHOULD THE FLAG BE?
+inline let pure_close_wp (a:Type) (b:Type) (wp:(b -> GTot (pure_wp a))) (is_wlp:bool) (p:pure_post a) = forall (b:b). wp b is_wlp p
+inline let pure_assert_p (a:Type) (p:Type) (wp:pure_wp a) (is_wlp:bool) (q:pure_post a) = (is_wlp \/ p) /\ ((~is_wlp \/ p) ==> wp is_wlp q)
+inline let pure_assume_p (a:Type) (p:Type) (wp:pure_wp a) (is_wlp:bool) (q:pure_post a) = p ==> wp is_wlp q
+inline let pure_null_wp  (a:Type) (is_wlp:bool) (p:pure_post a) = forall (x:a). p x
+inline let pure_trivial  (a:Type) (wp:pure_wp a) = wp false (fun (x:a) -> True) //TODO: WHAT SHOULD THE FLAG BE?
 
 total new_effect { (* The definition of the PURE effect is fixed; no user should ever change this *)
   PURE : a:Type -> wp:pure_wp a -> Effect
@@ -147,8 +155,10 @@ total new_effect { (* The definition of the PURE effect is fixed; no user should
 
 effect Pure (a:Type) (pre:pure_pre) (post:pure_post a) =
         PURE a
-             (fun (p:pure_post a) -> pre /\ (forall (x:a). pre /\ post x ==> p x)) // pure_wp
-effect Admit (a:Type) = PURE a (fun (p:pure_post a) -> True)
+             (fun (is_wlp:bool) (p:pure_post a) -> 
+	           (is_wlp \/ pre)
+		 /\ (forall (x:a). pre /\ post x ==> p x)) // pure_wp
+effect Admit (a:Type) = PURE a (fun (is_wlp:bool) (p:pure_post a) -> True)
 
 (* The primitive effect Tot is definitionally equal to an instance of PURE *)
 effect Tot (a:Type) = PURE a (pure_null_wp a)
@@ -165,7 +175,9 @@ effect GTot (a:Type) = GHOST a (pure_null_wp a)
 
 effect Ghost (a:Type) (pre:Type) (post:pure_post a) =
        GHOST a
-           (fun (p:pure_post a) -> pre /\ (forall (x:a). post x ==> p x))
+           (fun (is_wlp:bool) (p:pure_post a) -> 
+	         (is_wlp \/ pre)
+	       /\ (forall (x:a). post x ==> p x))
 
 assume new type int : Type0
 assume val op_AmpAmp             : bool -> bool -> Tot bool
@@ -226,68 +238,71 @@ sub_effect PURE ~> DIV  = purewp_id
 
 effect Div (a:Type) (pre:pure_pre) (post:pure_post a) =
        DIV a
-           (fun (p:pure_post a) -> pre /\ (forall a. pre /\ post a ==> p a)) (* WP *)
+           (fun (is_wlp:bool) (p:pure_post a) -> (is_wlp \/ pre) /\ (forall a. pre /\ post a ==> p a)) (* WP *)
 
 effect Dv (a:Type) =
-     DIV a (fun (p:pure_post a) -> (forall (x:a). p x))
+     DIV a (fun (is_wlp:bool) (p:pure_post a) -> (forall (x:a). p x))
 
 
 let st_pre_h  (heap:Type)          = heap -> GTot Type0
 let st_post_h (heap:Type) (a:Type) = a -> heap -> GTot Type0
-let st_wp_h   (heap:Type) (a:Type) = st_post_h heap a -> Tot (st_pre_h heap)
+let st_wp_h   (heap:Type) (a:Type) = bool -> st_post_h heap a -> Tot (st_pre_h heap)
 
 inline let st_return        (heap:Type) (a:Type)
-                            (x:a) (p:st_post_h heap a) =
+                            (x:a) (is_wlp:bool) (p:st_post_h heap a) =
      p x
 inline let st_bind_wp       (heap:Type) 
 			    (r1:range) 
 			    (a:Type) (b:Type)
                             (wp1:st_wp_h heap a)
                             (wp2:(a -> GTot (st_wp_h heap b)))
+			    (is_wlp:bool)
                             (p:st_post_h heap b) (h0:heap) =
      labeled r1 "push" unit
-     /\ wp1 (fun a h1 ->
+     /\ wp1 is_wlp (fun a h1 ->
        labeled r1 "pop" unit
-       /\ wp2 a p h1) h0
+       /\ wp2 a is_wlp p h1) h0
 inline let st_if_then_else  (heap:Type) (a:Type) (p:Type)
-                             (wp_then:st_wp_h heap a) (wp_else:st_wp_h heap a)
-                             (post:st_post_h heap a) (h0:heap) =
+                            (wp_then:st_wp_h heap a) (wp_else:st_wp_h heap a)
+                            (is_wlp:bool) (post:st_post_h heap a) (h0:heap) =
      l_ITE p
-        (wp_then post h0)
-	(wp_else post h0)
+        (wp_then is_wlp post h0)
+	(wp_else is_wlp post h0)
 inline let st_ite_wp        (heap:Type) (a:Type)
                             (wp:st_wp_h heap a)
+			    (is_wlp:bool)
                             (post:st_post_h heap a) (h0:heap) =
      (forall (a:a) (h:heap).
-           ~ (wp (fun a' h' -> a=!=a' \/ h=!=h') h0) ==> post a h)
-     /\ wp (fun _ _ -> True) h0
+           ~ (wp true (fun a' h' -> a=!=a' \/ h=!=h') h0) ==> post a h)
+     /\ (is_wlp \/ wp false (fun _ _ -> True) h0)
 
 inline let st_wp_binop      (heap:Type) (a:Type)
                              (wp1:st_wp_h heap a)
                              (op:(Type -> Type -> GTot Type))
                              (wp2:st_wp_h heap a)
+			     (is_wlp:bool)
                              (p:st_post_h heap a) (h:heap) =
-     op (wp1 p h) (wp2 p h)
+     op (wp1 is_wlp p h) (wp2 is_wlp p h)
 inline let st_wp_as_type    (heap:Type) (a:Type) (wp:st_wp_h heap a) =
-     (forall (p:st_post_h heap a) (h:heap). wp p h)
+     (forall (p:st_post_h heap a) (h:heap). wp false p h) //TODO: what should the flag be?
 inline let st_close_wp      (heap:Type) (a:Type) (b:Type)
                              (wp:(b -> GTot (st_wp_h heap a)))
-                             (p:st_post_h heap a) (h:heap) =
-     (forall (b:b). wp b p h)
+			     (is_wlp:bool) (p:st_post_h heap a) (h:heap) =
+     (forall (b:b). wp b is_wlp p h)
 inline let st_assert_p      (heap:Type) (a:Type) (p:Type)
-                             (wp:st_wp_h heap a)
-                             (q:st_post_h heap a) (h:heap) =
-     p /\ wp q h
+                            (wp:st_wp_h heap a) (is_wlp:bool)
+                            (q:st_post_h heap a) (h:heap) =
+     (is_wlp \/ p) /\ ((~is_wlp \/ p) ==> wp is_wlp q h)
 inline let st_assume_p      (heap:Type) (a:Type) (p:Type)
-                             (wp:st_wp_h heap a)
-                             (q:st_post_h heap a) (h:heap) =
-     p ==> wp q h
-inline let st_null_wp       (heap:Type) (a:Type)
-                             (p:st_post_h heap a) (h:heap) =
+                            (wp:st_wp_h heap a) (is_wlp:bool)
+                            (q:st_post_h heap a) (h:heap) =
+     p ==> wp is_wlp q h
+inline let st_null_wp       (heap:Type) (a:Type) (is_wlp:bool)
+                            (p:st_post_h heap a) (h:heap) =
      (forall (x:a) (h:heap). p x h)
 inline let st_trivial       (heap:Type) (a:Type)
-                             (wp:st_wp_h heap a) =
-     (forall h0. wp (fun r h1 -> True) h0)
+                            (wp:st_wp_h heap a) =
+     (forall h0. wp false (fun r h1 -> True) h0) //TODO: WHAT should the flag be?
 
 new_effect {
   STATE_h (heap:Type) : result:Type -> wp:st_wp_h heap result -> Effect
@@ -307,36 +322,37 @@ new_effect {
 (* Effect EXCEPTION *)
 let ex_pre  = Type0
 let ex_post (a:Type) = result a -> GTot Type0
-let ex_wp   (a:Type) = ex_post a -> GTot ex_pre
-inline let ex_return   (a:Type) (x:a) (p:ex_post a) : GTot Type0 = p (V x)
+let ex_wp   (a:Type) = bool -> ex_post a -> GTot ex_pre
+inline let ex_return   (a:Type) (x:a) (is_wlp:bool) (p:ex_post a) : GTot Type0 = p (V x)
 inline let ex_bind_wp (r1:range) (a:Type) (b:Type)
-		       (wp1:ex_wp a)
-		       (wp2:(a -> GTot (ex_wp b))) (p:ex_post b)
+		      (wp1:ex_wp a) (wp2:(a -> GTot (ex_wp b))) 
+		      (is_wlp:bool) (p:ex_post b)
          : GTot Type0 =
-   (forall (rb:result b). p rb \/ wp1 (fun ra1 -> l_ITE (is_V ra1)
-						(wp2 (V.v ra1) (fun rb2 -> rb2=!=rb))
-						(ra1 =!= rb)))
-   /\ labeled r1 "push" unit
-   /\ wp1 (fun ra1 ->  
-     labeled r1 "pop" unit
-     /\ (is_V ra1 ==> wp2 (V.v ra1) (fun rb2 -> True)))
+   (forall (rb:result b). p rb \/ wp1 true (fun ra1 -> l_ITE (is_V ra1)
+						    (wp2 (V.v ra1) true (fun rb2 -> rb2=!=rb))
+						    (ra1 =!= rb)))
+   /\ (is_wlp 
+      \/ (labeled r1 "push" unit
+         /\ wp1 false (fun ra1 ->  
+	   labeled r1 "pop" unit
+	   /\ (is_V ra1 ==> wp2 (V.v ra1) false (fun rb2 -> True)))))
 
-inline let ex_ite_wp (a:Type) (wp:ex_wp a) (post:ex_post a) =
-    (forall (x:result a). post x \/ wp (fun x' -> x=!=x'))
-    /\ wp (fun _ -> True)
+inline let ex_ite_wp (a:Type) (wp:ex_wp a) (is_wlp:bool) (post:ex_post a) =
+    (forall (x:result a). post x \/ wp true (fun x' -> x=!=x'))
+    /\ (is_wlp \/ wp false (fun _ -> True))
 
-inline let ex_if_then_else (a:Type) (p:Type) (wp_then:ex_wp a) (wp_else:ex_wp a) (post:ex_post a) =
+inline let ex_if_then_else (a:Type) (p:Type) (wp_then:ex_wp a) (wp_else:ex_wp a) (is_wlp:bool) (post:ex_post a) =
    l_ITE p
-       (wp_then post)
-       (wp_else post)
-inline let ex_wp_binop (a:Type) (wp1:ex_wp a) (op:(Type -> Type -> GTot Type)) (wp2:ex_wp a) (p:ex_post a) =
-   op (wp1 p) (wp2 p)
-inline let ex_wp_as_type (a:Type) (wp:ex_wp a) = (forall (p:ex_post a). wp p)
-inline let ex_close_wp (a:Type) (b:Type) (wp:(b -> GTot (ex_wp a))) (p:ex_post a) = (forall (b:b). wp b p)
-inline let ex_assert_p (a:Type) (q:Type) (wp:ex_wp a) (p:ex_post a) = (q /\ wp p)
-inline let ex_assume_p (a:Type) (q:Type) (wp:ex_wp a) (p:ex_post a) = (q ==> wp p)
-inline let ex_null_wp (a:Type) (p:ex_post a) = (forall (r:result a). p r)
-inline let ex_trivial (a:Type) (wp:ex_wp a) = wp (fun r -> True)
+       (wp_then is_wlp post)
+       (wp_else is_wlp post)
+inline let ex_wp_binop (a:Type) (wp1:ex_wp a) (op:(Type -> Type -> GTot Type)) (wp2:ex_wp a) (is_wlp:bool) (p:ex_post a) =
+   op (wp1 is_wlp p) (wp2 is_wlp p)
+inline let ex_wp_as_type (a:Type) (wp:ex_wp a) = (forall (p:ex_post a). wp false p) //TODO: what's the flag?
+inline let ex_close_wp (a:Type) (b:Type) (wp:(b -> GTot (ex_wp a))) (is_wlp:bool) (p:ex_post a) = (forall (b:b). wp b is_wlp p)
+inline let ex_assert_p (a:Type) (p:Type) (wp:ex_wp a) (is_wlp:bool) (q:ex_post a) = (is_wlp \/ p) /\ ((~is_wlp \/ p) ==> wp is_wlp q)
+inline let ex_assume_p (a:Type) (p:Type) (wp:ex_wp a) (is_wlp:bool) (q:ex_post a) = p ==> wp is_wlp q
+inline let ex_null_wp (a:Type) (is_wlp:bool) (p:ex_post a) = (forall (r:result a). p r)
+inline let ex_trivial (a:Type) (wp:ex_wp a) = wp false (fun r -> True) //TODO: what's the flag?
 
 new_effect {
   EXN : result:Type -> wp:ex_wp result -> Effect
@@ -355,59 +371,61 @@ new_effect {
 }
 effect Exn (a:Type) (pre:ex_pre) (post:ex_post a) =
        EXN a
-         (fun (p:ex_post a) -> pre /\ (forall (r:result a). (pre /\ post r) ==> p r)) (* WP *)
+         (fun (is_wlp:bool) (p:ex_post a) -> (is_wlp \/ pre) /\ (forall (r:result a). (pre /\ post r) ==> p r)) (* WP *)
 
-inline let lift_div_exn (a:Type) (wp:pure_wp a) (p:ex_post a) = wp (fun a -> p (V a))
+inline let lift_div_exn (a:Type) (wp:pure_wp a) (is_wlp:bool) (p:ex_post a) = wp is_wlp (fun a -> p (V a))
 sub_effect DIV ~> EXN = lift_div_exn
 effect Ex (a:Type) = Exn a True (fun v -> True)
 
 let all_pre_h  (h:Type)           = h -> GTot Type0
 let all_post_h (h:Type) (a:Type)  = result a -> h -> GTot Type0
-let all_wp_h   (h:Type) (a:Type)  = all_post_h h a -> Tot (all_pre_h h)
+let all_wp_h   (h:Type) (a:Type)  = bool -> all_post_h h a -> Tot (all_pre_h h)
 
 inline let all_ite_wp (heap:Type) (a:Type)
-                      (wp:all_wp_h heap a)
+                      (wp:all_wp_h heap a) (is_wlp:bool)
                       (post:all_post_h heap a) (h0:heap) =
-     wp (fun _ _ -> True) h0 /\
-     (forall (r:result a) (h:heap). wp (fun r' h' -> r=!=r' \/ h=!=h') h0 \/ post r h)
-
-inline let all_return  (heap:Type) (a:Type) (x:a) (p:all_post_h heap a) = p (V x)
+     (forall (r:result a) (h:heap). wp true (fun r' h' -> r=!=r' \/ h=!=h') h0 \/ post r h)
+     /\ (is_wlp \/ wp false (fun _ _ -> True) h0)
+     
+inline let all_return  (heap:Type) (a:Type) (x:a) (is_wlp:bool) (p:all_post_h heap a) = p (V x)
 inline let all_bind_wp (heap:Type) (r1:range) (a:Type) (b:Type)
                        (wp1:all_wp_h heap a)
                        (wp2:(a -> GTot (all_wp_h heap b)))
+		       (is_wlp:bool)
                        (p:all_post_h heap b) (h0:heap) : GTot Type0 =
    labeled r1 "push" unit
-   /\ wp1 (fun ra h1 -> 
+   /\ wp1 is_wlp (fun ra h1 -> 
        labeled r1 "pop" unit
-       /\ (is_V ra ==> wp2 (V.v ra) p h1)) h0
+       /\ (is_V ra ==> wp2 (V.v ra) is_wlp p h1)) h0
 
 inline let all_if_then_else (heap:Type) (a:Type) (p:Type)
-                             (wp_then:all_wp_h heap a) (wp_else:all_wp_h heap a)
-                             (post:all_post_h heap a) (h0:heap) =
+                            (wp_then:all_wp_h heap a) (wp_else:all_wp_h heap a)
+                            (is_wlp:bool) (post:all_post_h heap a) (h0:heap) =
    l_ITE p
-       (wp_then post h0)
-       (wp_else post h0)
+       (wp_then is_wlp post h0)
+       (wp_else is_wlp post h0)
 inline let all_wp_binop (heap:Type) (a:Type)
                          (wp1:all_wp_h heap a) (op:(Type -> Type -> GTot Type))
-                         (wp2:all_wp_h heap a) (p:all_post_h heap a) (h:heap) =
-     op (wp1 p h) (wp2 p h)
+                         (wp2:all_wp_h heap a) (is_wlp:bool) (p:all_post_h heap a) (h:heap) =
+     op (wp1 is_wlp p h) (wp2 is_wlp p h)
 inline let all_wp_as_type (heap:Type) (a:Type) (wp:all_wp_h heap a) =
-    (forall (p:all_post_h heap a) (h:heap). wp p h)
+    (forall (p:all_post_h heap a) (h:heap). wp false p h) //TODO: what's the flag?
 inline let all_close_wp (heap:Type) (a:Type) (b:Type)
-                         (wp:(b -> GTot (all_wp_h heap a)))
-                         (p:all_post_h heap a) (h:heap) =
-    (forall (b:b). wp b p h)
+                        (wp:(b -> GTot (all_wp_h heap a)))
+		        (is_wlp:bool)
+                        (p:all_post_h heap a) (h:heap) =
+    (forall (b:b). wp b is_wlp p h)
 inline let all_assert_p (heap:Type) (a:Type) (p:Type)
-                         (wp:all_wp_h heap a) (q:all_post_h heap a) (h:heap) =
-    p /\ wp q h
+                        (wp:all_wp_h heap a) (is_wlp:bool) (q:all_post_h heap a) (h:heap) =
+    (is_wlp \/ p) /\ ((~is_wlp \/ p) ==> wp is_wlp q h)
 inline let all_assume_p (heap:Type) (a:Type) (p:Type)
-                         (wp:all_wp_h heap a) (q:all_post_h heap a) (h:heap) =
-    p ==> wp q h
-inline let all_null_wp (heap:Type) (a:Type)
-                        (p:all_post_h heap a) (h0:heap) =
+                        (wp:all_wp_h heap a) (is_wlp:bool) (q:all_post_h heap a) (h:heap) =
+    p ==> wp is_wlp q h
+inline let all_null_wp (heap:Type) (a:Type) (is_wlp:bool)
+                       (p:all_post_h heap a) (h0:heap) =
     (forall (a:result a) (h:heap). p a h)
 inline let all_trivial (heap:Type) (a:Type) (wp:all_wp_h heap a) =
-    (forall (h0:heap). wp (fun r h1 -> True) h0)
+    (forall (h0:heap). wp false (fun r h1 -> True) h0) //TODO: what's the flag?
 
 new_effect {
   ALL_h (heap:Type) : a:Type -> wp:all_wp_h heap a -> Effect
@@ -517,8 +535,8 @@ type dtuple4 (a:Type)
            -> _4:d _1 _2 _3
            -> dtuple4 a b c d
 
-let as_requires (#a:Type) (wp:pure_wp a)  = wp (fun x -> True)
-let as_ensures  (#a:Type) (wp:pure_wp a) (x:a) = ~ (wp (fun y -> (y=!=x)))
+let as_requires (#a:Type) (wp:pure_wp a)  = wp false (fun x -> True)
+let as_ensures  (#a:Type) (wp:pure_wp a) (x:a) = ~ (wp true (fun y -> (y=!=x)))
 
 val fst : ('a * 'b) -> Tot 'a
 let fst x = Mktuple2._1 x
