ulib/FStar.TwoLevelHeap.fst
@@ -27,11 +27,11 @@ effect State (a:Type) (wp:st_wp a) =
        STATE a wp
 effect ST (a:Type) (pre:st_pre) (post: (t -> Tot (st_post a))) =
        STATE a
-             (fun (p:st_post a) (h:t) -> pre h /\ (forall a h1. pre h /\ post h a h1 ==> p a h1)) (* WP *)
+             (fun (is_wlp:bool) (p:st_post a) (h:t) -> (is_wlp \/ pre h) /\ (forall a h1. pre h /\ post h a h1 ==> p a h1)) (* WP *)
 effect St (a:Type) =
        ST a (fun h -> True) (fun h0 r h1 -> True)
 sub_effect
-  DIV   ~> STATE = fun (a:Type) (wp:pure_wp a) (p:st_post a) (h:t) -> wp (fun a -> p a h)
+  DIV   ~> STATE = fun (a:Type) (wp:pure_wp a) (is_wlp:bool) (p:st_post a) (h:t) -> wp is_wlp (fun a -> p a h)
 
 type rref (id:rid) (a:Type) = ref a
 val as_ref : #a:Type -> #id:rid -> r:rref id a -> Tot (ref a)
